SporkProofs/Syntax.lean
@@ -35,14 +35,22 @@ inductive Code where
   | ite (cond : Atom) (bthen : Cont) (belse : Cont)
   | call (f : FuncIdx) (args : List Var) (bret : Cont)
   | retn (args : List Var)
-  | spork (bbody : Cont) (fspwn : FuncIdx) (args : List Var)
+  | spork (n : Nat) (bbody : Cont) (bspwn : Cont)
   | spoin (bunpr : Cont) (bprom : Cont)
+  | join (bsync : Cont)
+  | exit (args : List Var)
 
-abbrev SporkSig := List Nat
+--abbrev SporkSig := List Nat
+-- Obligation to return, exit, spoin, or join
+inductive Oblg where
+  | retn (n : Nat)
+  | exit (n : Nat)
+  | spoin (σ : Oblg) (n : Nat)
+  | join (σ : Oblg) (n : Nat)
 
 -- block with `arity` args and nested under `sporks`
 inductive BlockSig where
-  | mk (arity : Nat) (sporkNest : SporkSig)
+  | mk (arity : Nat) (oblg : Oblg)
 
 inductive Block where
   | mk (bsig : BlockSig) (code : Code)
@@ -54,35 +62,104 @@ inductive Func where
   | mk (fsig : FuncSig) (blocks : List Block)
 
 inductive Program where
-  | mk (funs : List Func)
+  | mk (funs : List Func) (main: List Block)
 
 abbrev Scope := Nat
 abbrev FuncSigs := List FuncSig
 abbrev BlockSigs := List BlockSig
 
+namespace Oblg
+--  @[simp] abbrev spoin
+  deriving instance DecidableEq for Oblg
+
+  inductive isRetn : Oblg -> Prop where
+    | mk (n : Nat) : (retn n).isRetn
+  inductive isExit : Oblg -> Prop where
+    | mk (n : Nat) : (exit n).isExit
+  inductive isSpoin : Oblg -> Prop where
+    | mk (σ : Oblg) (n : Nat) : (σ.spoin n).isSpoin
+  inductive isJoin : Oblg -> Prop where
+    | mk (σ : Oblg) (n : Nat) : (σ.join n).isJoin
+  -- inductive isRetnN : Oblg -> Nat -> Prop where
+  --   | mk (n : Nat) : (retn n).isRetnN n
+  -- inductive isExitN : Oblg -> Nat -> Prop where
+  --   | mk (n : Nat) : (exit n).isExitN n
+
+  instance : {σ : Oblg} -> Decidable σ.isRetn := by
+    intro σ; cases σ <;> try exact .isFalse (by intro; contradiction)
+    · case retn n => exact .isTrue (.mk n)
+  instance : {σ : Oblg} -> Decidable σ.isExit := by
+    intro σ; cases σ <;> try exact .isFalse (by intro; contradiction)
+    · case exit n => exact .isTrue (.mk n)
+  instance : {σ : Oblg} -> Decidable σ.isSpoin := by
+    intro σ; cases σ <;> try exact .isFalse (by intro; contradiction)
+    · case spoin σ n => exact .isTrue (.mk σ n)
+  instance : {σ : Oblg} -> Decidable σ.isJoin := by
+    intro σ; cases σ <;> try exact .isFalse (by intro; contradiction)
+    · case join σ n => exact .isTrue (.mk σ n)
+  -- instance : {σ : Oblg} -> {n : Nat} -> Decidable (σ.isRetnN n) := by
+  --   intro σ n; cases σ <;> try exact .isFalse (by intro; contradiction)
+  --   · case retn n' => exact decidable_of_iff (n = n')
+  --                       ⟨λ h => by rw[h]; exact .mk n', λ | .mk n'' => rfl⟩
+  -- instance : {σ : Oblg} -> {n : Nat} -> Decidable (σ.isExitN n) := by
+  --   intro σ n; cases σ <;> try exact .isFalse (by intro; contradiction)
+  --   · case exit n' => exact decidable_of_iff (n = n')
+  --                       ⟨λ h => by rw[h]; exact .mk n', λ | .mk n'' => rfl⟩
+
+  @[simp] abbrev getRetn : (σ : Oblg) -> σ.isRetn -> Nat
+    | retn n, _ => n
+  @[simp] abbrev getExit : (σ : Oblg) -> σ.isExit -> Nat
+    | exit n, _ => n
+  @[simp] abbrev getSpoin : (σ : Oblg) -> σ.isSpoin -> Oblg × Nat
+    | spoin σ n, _ => ⟨σ, n⟩
+  @[simp] abbrev getJoin : (σ : Oblg) -> σ.isJoin -> Oblg × Nat
+    | join σ n, _ => ⟨σ, n⟩
+
+  @[simp] abbrev head : Oblg -> Nat
+    | retn n => n
+    | exit n => n
+    | spoin _σ n => n
+    | join _σ n => n
+  @[simp] abbrev tail : Oblg -> Oblg
+    | retn n => retn n
+    | exit n => exit n
+    | spoin σ _n => σ
+    | join σ _n => σ
+  
+end Oblg
+
 namespace BlockSig
-  @[simp] abbrev arity | mk a _ss => a
-  @[simp] abbrev sporkNest | mk _a ss => ss
-  @[simp] abbrev bind | mk a ss => mk a.succ ss
-  @[simp] abbrev spork | mk a ss, s => mk a (s :: ss)
-  @[simp] abbrev spoin | mk a ss => mk a ss.tail
+  @[simp] abbrev arity | mk a _σ => a
+  @[simp] abbrev oblg | mk _a σ => σ
+  @[simp] abbrev bind | mk a σ => mk a.succ σ
+  @[simp] abbrev retn | mk a _σ, n => mk a (Oblg.retn n)
+  @[simp] abbrev exit | mk a _σ, n => mk a (Oblg.exit n)
+  @[simp] abbrev spoin | mk a σ, n => mk a (σ.spoin n)
+  @[simp] abbrev join | mk a σ, n => mk a (σ.join n)
+  @[simp] abbrev head | mk _a σ => σ.head
+  @[simp] abbrev tail | mk a σ => mk a σ.tail
+  @[simp] abbrev binds | mk a σ, b => mk (a + b) σ
+--  @[simp] abbrev join
+
+  -- @[simp] abbrev spork | mk a σ, s => mk a (SporkSig.spwn σ s)
+  -- @[simp] abbrev spoin | mk a σ => mk a σ.tail
 
   deriving instance DecidableEq for BlockSig
 
-  @[simp] def add (a b : BlockSig) :=
-    mk (a.arity + b.arity) (a.sporkNest ++ b.sporkNest)
+  -- @[simp] def add (a b : BlockSig) :=
+  --   mk (a.arity + b.arity) (a.sporkNest ++ b.sporkNest)
 
-  instance : Add BlockSig where
-    add := add
+  -- instance : Add BlockSig where
+  --   add := add
 
-  @[simp] theorem add_arity (a b : BlockSig) : (a + b).arity = a.arity + b.arity :=
-    by simp
-  @[simp] theorem add_sporkNest (a b : BlockSig) : (a + b).sporkNest = a.sporkNest ++ b.sporkNest :=
-    by simp
-  @[simp] theorem add_unfolded (a a' sn sn') : (mk a sn) + (mk a' sn') = mk (a + a') (sn ++ sn') :=
-    rfl
-  @[simp] theorem add_zero : (a : BlockSig) -> (a + .mk 0 []) = a
-    | .mk arity sn => by simp
+  -- @[simp] theorem add_arity (a b : BlockSig) : (a + b).arity = a.arity + b.arity :=
+  --   by simp
+  -- @[simp] theorem add_sporkNest (a b : BlockSig) : (a + b).sporkNest = a.sporkNest ++ b.sporkNest :=
+  --   by simp
+  -- @[simp] theorem add_unfolded (a a' sn sn') : (mk a sn) + (mk a' sn') = mk (a + a') (sn ++ sn') :=
+  --   rfl
+  -- @[simp] theorem add_zero : (a : BlockSig) -> (a + .mk 0 []) = a
+  --   | .mk arity sn => by simp
 end BlockSig
 
 namespace FuncSig
@@ -97,19 +174,6 @@ namespace Var
 
   @[simp] abbrev inc | mk v, n => mk (v + n)
 
-  inductive WF (Γ : Scope) (v : Var) : Prop where
-    | mk : v.idx < Γ -> v.WF Γ
-
-  namespace WF
-    theorem idx {Γ : Scope} {v : Var} : v.WF Γ -> v.idx < Γ | .mk idx => idx
-
-    instance {Γ : Scope} {v : Var} : Decidable (v.WF Γ) :=
-      decidable_of_iff (v.idx < Γ) ⟨(⟨·⟩), (·.1)⟩
-
-    theorem weakening {Γ Γ'} {v : Var} (wf : v.WF Γ) : v.WF (Γ + Γ') :=
-      .mk (Nat.lt_add_right Γ' wf.idx)
-  end WF
-  
   deriving instance DecidableEq for Var
 
   instance {n} : OfNat Var n where
@@ -120,22 +184,24 @@ namespace Var
     coe := idx
 end Var
 
-namespace Atom
-  inductive WF (Γ : Scope) : Atom -> Prop where
-    | val {v : Val} : (val v).WF Γ
-    | var {v : Var} : v.WF Γ -> (var v).WF Γ
+namespace Var
+  inductive WF (Γ : Scope) (v : Var) : Prop where
+    | mk : v.idx < Γ -> v.WF Γ
 
   namespace WF
-    instance {Γ : Scope} : (a : Atom) -> Decidable (a.WF Γ)
-      | .val _v => isTrue val
-      | .var v => decidable_of_iff (v.WF Γ) ⟨var, λ (var v) => v⟩
+    notation (name := wfnotation) Γ:arg " ⊢ " v:arg " WF-var" => WF Γ v
 
-    theorem vwf {Γ : Scope} {v : Var} : (Atom.var v).WF Γ -> v.WF Γ | .var wf => wf
+    theorem idx {Γ : Scope} {v : Var} : Γ ⊢ v WF-var -> v.idx < Γ | .mk idx => idx
 
-    theorem weakening {Γ Γ'} {a : Atom} : a.WF Γ -> a.WF (Γ + Γ')
-      | .val => .val
-      | .var wf => .var wf.weakening
+    instance {Γ : Scope} {v : Var} : Decidable (Γ ⊢ v WF-var) :=
+      decidable_of_iff (v.idx < Γ) ⟨(⟨·⟩), (·.1)⟩
+
+    theorem weakening {Γ Γ'} {v : Var} (wf : Γ ⊢ v WF-var) : (Γ + Γ') ⊢ v WF-var :=
+      .mk (Nat.lt_add_right Γ' wf.idx)
   end WF
+end Var
+
+namespace Atom
   deriving instance DecidableEq for Atom
 end Atom
 
@@ -147,72 +213,182 @@ namespace Bop
   deriving instance DecidableEq for Bop
 end Bop
 
-namespace Expr  
-  inductive WF (Γ : Scope) : Expr -> Prop where
-    | nop {a : Atom} : a.WF Γ -> (nop a).WF Γ
-    | uop {o : Uop} {a : Atom} : a.WF Γ -> (uop o a).WF Γ
-    | bop {o : Bop} {a b : Atom} : a.WF Γ -> b.WF Γ -> (bop o a b).WF Γ
-
-  namespace WF
-    instance {Γ : Scope} : (e : Expr) -> Decidable (e.WF Γ)
-      | .nop a => decidable_of_iff (a.WF Γ)
-          ⟨nop, λ (nop a) => a⟩
-      | .uop _o a => decidable_of_iff (a.WF Γ)
-          ⟨uop, λ (uop wf) => wf⟩
-      | .bop _o a b => decidable_of_iff (a.WF Γ ∧ b.WF Γ)
-          ⟨And.elim bop, λ (bop a b) => ⟨a, b⟩⟩
-
-    theorem weakening {Γ Γ'} {e : Expr} : e.WF Γ -> e.WF (Γ + Γ')
-      | .nop a => .nop a.weakening
-      | .uop a => .uop a.weakening
-      | .bop a b => .bop a.weakening b.weakening
-  end WF
-
+namespace Expr
   deriving instance DecidableEq for Expr
 end Expr
 
 namespace Cont
+  deriving instance DecidableEq for Cont
+
   @[simp] abbrev b | mk b _args => b
   @[simp] abbrev args | mk _b args => args
+end Cont
 
+namespace Code
+  deriving instance DecidableEq for Code
+
+  @[simp] def split : Code -> List Expr × (c : Code) ×' (∀ e, ∀ c', c ≠ .stmt e c')
+    | stmt e c => let (es, cp) := c.split
+                  (e :: es, cp)
+    | goto bnext => ([], ⟨goto bnext, by intros e c; simp⟩)
+    | ite e bthen belse => ([], ⟨ite e bthen belse, by intros e c; simp⟩)
+    | call g args bret => ([], ⟨call g args bret, by intros e c; simp⟩)
+    | retn args => ([], ⟨retn args, by intros e c; simp⟩)
+    | spork n bbody bspwn => ([], ⟨spork n bbody bspwn, by intros e c; simp⟩)
+    | spoin bunpr bprom => ([], ⟨spoin bunpr bprom, by intros e c; simp⟩)
+    | join bsync => ([], ⟨join bsync, by intros e c; simp⟩)
+    | exit args => ([], ⟨exit args, by intros e c; simp⟩)
+
+  @[simp] def merge : List Expr -> Code -> Code
+    | [], c => c
+    | e :: es, c => stmt e (merge es c)
+
+  @[simp] theorem merge_split {c e c' p} (q : split c = (e, ⟨c', p⟩)) : merge e c' = c := by
+    cases c <;> try (cases e <;> simp_all)
+    · case stmt e' es' e'' es'' =>
+      exact merge_split (Prod.ext q.1.2 q.2)
+end Code
+
+namespace Block
+  @[simp] abbrev bsig | mk bsig _code => bsig
+  @[simp] abbrev code | mk _bsig code => code
+
+  deriving instance DecidableEq for Block
+
+  instance : Inhabited Block where
+    default := mk ⟨0, .retn 0⟩ (.retn [])
+end Block
+
+
+namespace Func
+  @[simp] abbrev fsig | mk fsig _blocks => fsig
+  @[simp] abbrev blocks | mk _fsig blocks => blocks
+  @[simp] abbrev bsigs : Func -> BlockSigs | mk _fsig blocks => blocks.map (·.bsig)
+  @[simp] abbrev size | mk _fsig blocks => blocks.length
+
+  @[simp] theorem size_eq_bsigs_length (f : Func) : f.bsigs.length = f.size :=
+    by simp
+
+  deriving instance DecidableEq for Func
+
+  instance : Inhabited Func where
+    default := mk ⟨0, 0⟩ default
+
+  instance : GetElem Func BlockIdx Block (λ f b => b < f.blocks.length) where
+    getElem f b p := f.blocks[b]
+end Func
+
+namespace Program
+  @[simp] abbrev funs | mk funs _main => funs
+  @[simp] abbrev main | mk _funs main => main
+  @[simp] abbrev fsigs : Program -> FuncSigs
+    | mk funs _main => funs.map (·.fsig)
+  @[simp] abbrev size : Program -> Nat
+    | mk funs _main => funs.length
+
+  @[simp] theorem size_eq_fsigs_length (P : Program) : P.fsigs.length = P.size :=
+    by simp
+
+  deriving instance DecidableEq for Program
+
+  instance : GetElem Program FuncIdx Func (λ P f => f < P.size) where
+    getElem P f p := P.funs[f]
+end Program
+
+/- ==================== Well-Formedness Rules ==================== -/
+
+namespace Atom
+  inductive WF (Γ : Scope) : Atom -> Prop where
+    | val {v : Val} : (val v).WF Γ
+    | var {v : Var} : Γ ⊢ v WF-var -> (var v).WF Γ
+
+  namespace WF
+    notation (name := wfnotation) Γ:arg " ⊢ " a:arg " WF-atom" => WF Γ a
+
+    instance {Γ : Scope} : (a : Atom) -> Decidable (Γ ⊢ a WF-atom)
+      | .val _v => isTrue val
+      | .var v => decidable_of_iff (Γ ⊢ v WF-var) ⟨var, λ (var v) => v⟩
+
+    theorem vwf {Γ : Scope} {v : Var} : Γ ⊢ (Atom.var v) WF-atom -> Γ ⊢ v WF-var
+      | .var wf => wf
+
+    theorem weakening {Γ Γ'} {a : Atom} : Γ ⊢ a WF-atom -> (Γ + Γ') ⊢ a WF-atom
+      | .val => .val
+      | .var wf => .var wf.weakening
+  end WF
+end Atom
+
+namespace Expr  
+  inductive WF (Γ : Scope) : Expr -> Prop where
+    | nop {a : Atom} : Γ ⊢ a WF-atom -> (nop a).WF Γ
+    | uop {o : Uop} {a : Atom} : Γ ⊢ a WF-atom -> (uop o a).WF Γ
+    | bop {o : Bop} {a b : Atom} : Γ ⊢ a WF-atom -> Γ ⊢ b WF-atom -> (bop o a b).WF Γ
+
+  namespace WF
+    notation (name := wfnotation) Γ:arg " ⊢ " e:arg " WF-expr" => WF Γ e
+
+    instance {Γ : Scope} : (e : Expr) -> Decidable (Γ ⊢ e WF-expr)
+      | .nop a => decidable_of_iff (Γ ⊢ a WF-atom)
+          ⟨nop, λ (nop a) => a⟩
+      | .uop _o a => decidable_of_iff (Γ ⊢ a WF-atom)
+          ⟨uop, λ (uop wf) => wf⟩
+      | .bop _o a b => decidable_of_iff (Γ ⊢ a WF-atom ∧ Γ ⊢ b WF-atom)
+          ⟨And.elim bop, λ (bop a b) => ⟨a, b⟩⟩
+
+    theorem weakening {Γ Γ'} {e : Expr} : Γ ⊢ e WF-expr -> (Γ + Γ') ⊢ e WF-expr
+      | .nop a => .nop a.weakening
+      | .uop a => .uop a.weakening
+      | .bop a b => .bop a.weakening b.weakening
+  end WF
+end Expr
+
+namespace Cont
   -- a continuation that takes `bsig.arity + rets` args
   inductive WFRets (bsigs : BlockSigs) (bsig : BlockSig) (rets : Nat) (b : Cont) : Prop where
     | mk (_ : b.b < bsigs.length)
-         (_ : bsigs[b.b] = ⟨b.args.length + rets, bsig.sporkNest⟩)
-         (_ : IVec (·.WF bsig.arity) b.args)
+         (_ : bsigs[b.b] = ⟨b.args.length + rets, bsig.oblg⟩)
+         (_ : IVec (bsig.arity ⊢ · WF-var) b.args)
 
   inductive WF (bsigs : BlockSigs) (bsig : BlockSig) (b : Cont) : Prop where
     | mk (_ : b.b < bsigs.length)
-         (_ : bsigs[b.b] = ⟨b.args.length, bsig.sporkNest⟩)
-         (_ : IVec (·.WF bsig.arity) b.args)
+         (_ : bsigs[b.b] = ⟨b.args.length, bsig.oblg⟩)
+         (_ : IVec (bsig.arity ⊢ · WF-var) b.args)
+
+  namespace WFRets
+    notation (name := notationwf) bsigs:arg " ; " bsig:arg " ⊢ " b:arg " ( " rets:arg " )" " WF-cont" => WFRets bsigs bsig rets b
+  end WFRets
+  namespace WF
+    notation (name := notationwf) bsigs:arg " ; " bsig:arg " ⊢ " b:arg " WF-cont" => WF bsigs bsig b
+  end WF
 
   namespace WFRets
     instance {bsigs : BlockSigs} {bsig : BlockSig} {b : Cont} :
-             Coe (WFRets bsigs bsig 0 b) (WF bsigs bsig b) where
+             Coe (bsigs; bsig ⊢ b(0) WF-cont) (bsigs; bsig ⊢ b WF-cont) where
       coe := λ ⟨bwf, blen, argswf⟩ => ⟨bwf, blen, argswf⟩
 
-    instance {bsigs : BlockSigs} {bsig : BlockSig} {rets : Nat} {b : Cont} : Decidable (b.WFRets bsigs bsig rets) :=
+    instance wf {bsigs : BlockSigs} {bsig : BlockSig} {rets : Nat} {b : Cont} :
+                Decidable (bsigs; bsig ⊢ b(rets) WF-cont) :=
       dite (b.b < bsigs.length)
         (λ t => decidable_of_iff
-                  ((bsigs[b.b] = ⟨b.args.length + rets, bsig.sporkNest⟩) ∧
-                   IVec (·.WF bsig.arity) b.args)
+                  ((bsigs[b.b] = ⟨b.args.length + rets, bsig.oblg⟩) ∧
+                   IVec (bsig.arity ⊢ · WF-var) b.args)
                   ⟨λ ⟨p1, p2⟩ => ⟨t, p1, p2⟩,
                    λ ⟨_, p1, p2⟩ => ⟨p1, p2⟩⟩)
         (λ f => isFalse (f ∘ (λ ⟨p, _, _⟩ => p)))
 
-    abbrev cast0 {bsigs bsig b} : WFRets bsigs bsig 0 b -> WF bsigs bsig b
+    abbrev cast0 {bsigs bsig b} : bsigs; bsig ⊢ b(0) WF-cont -> bsigs; bsig ⊢ b WF-cont
       | ⟨a, b, c⟩ => ⟨a, b, c⟩
-    theorem blt {bsigs bsig rets b} (wf : WFRets bsigs bsig rets b) :
+    theorem blt {bsigs bsig rets b} (wf : bsigs; bsig ⊢ b(rets) WF-cont) :
                 b.b < bsigs.length := wf.1
-    theorem bsig {bsigs bsig rets b} (wf : WFRets bsigs bsig rets b) :
-                 bsigs[b.b]'wf.blt = ⟨b.args.length + rets, bsig.sporkNest⟩ := wf.2
-    theorem args {bsigs bsig rets b} (wf : WFRets bsigs bsig rets b) :
-                 IVec (·.WF bsig.arity) b.args := wf.3
+    theorem bsig {bsigs bsig rets b} (wf : bsigs; bsig ⊢ b(rets) WF-cont) :
+                 bsigs[b.b]'wf.blt = ⟨b.args.length + rets, bsig.oblg⟩ := wf.2
+    theorem args {bsigs bsig rets b} (wf : bsigs; bsig ⊢ b(rets) WF-cont) :
+                 IVec (bsig.arity ⊢ · WF-var) b.args := wf.3
 
     theorem weakening_bsigs
             {bsigs bsigs' bsig ret b} :
-            WFRets bsigs bsig ret b ->
-            WFRets (bsigs ++ bsigs') bsig ret b
+            bsigs; bsig ⊢ b(ret) WF-cont ->
+            (bsigs ++ bsigs'); bsig ⊢ b(ret) WF-cont
       | mk blt bsigb args =>
         mk (List.length_append ▸ Nat.lt_add_right bsigs'.length blt)
            (List.getElem_append_left' blt bsigs' ▸ bsigb)
@@ -221,62 +397,61 @@ namespace Cont
 
   namespace WF
     instance {bsigs : BlockSigs} {bsig : BlockSig} {b : Cont} :
-             Coe (WF bsigs bsig b) (WFRets bsigs bsig 0 b) where
+             Coe (bsigs; bsig ⊢ b WF-cont) (bsigs; bsig ⊢ b(0) WF-cont) where
       coe := λ ⟨bwf, blen, argswf⟩ => ⟨bwf, blen, argswf⟩
 
-    instance {bsigs : BlockSigs} {bsig : BlockSig} {b : Cont} : Decidable (b.WF bsigs bsig) :=
+    instance wf {bsigs : BlockSigs} {bsig : BlockSig} {b : Cont} :
+                Decidable (bsigs; bsig ⊢ b WF-cont) :=
       decidable_of_iff (b.WFRets bsigs bsig 0) ⟨Coe.coe, Coe.coe⟩
 
-    abbrev cast0 {bsigs bsig b} : WF bsigs bsig b -> WFRets bsigs bsig 0 b
+    abbrev cast0 {bsigs bsig b} : bsigs; bsig ⊢ b WF-cont -> bsigs; bsig ⊢ b(0) WF-cont
       | ⟨a, b, c⟩ => ⟨a, b, c⟩
-    theorem blt {bsigs bsig b} (wf : WF bsigs bsig b) :
+    theorem blt {bsigs bsig b} (wf : bsigs; bsig ⊢ b WF-cont) :
                 b.b < bsigs.length := wf.1
-    theorem bsig {bsigs bsig b} (wf : WF bsigs bsig b) :
-                 bsigs[b.b]'wf.blt = ⟨b.args.length, bsig.sporkNest⟩ := wf.2
-    theorem args {bsigs bsig b} (wf : WF bsigs bsig b) :
-                 IVec (·.WF bsig.arity) b.args := wf.3
+    theorem bsig {bsigs bsig b} (wf : bsigs; bsig ⊢ b WF-cont) :
+                 bsigs[b.b]'wf.blt = ⟨b.args.length, bsig.oblg⟩ := wf.2
+    theorem args {bsigs bsig b} (wf : bsigs; bsig ⊢ b WF-cont) :
+                 IVec (bsig.arity ⊢ · WF-var) b.args := wf.3
 
     theorem weakening_bsigs
             {bsigs bsigs' bsig b}
-            (wf : WF bsigs bsig b) :
-            WF (bsigs ++ bsigs') bsig b :=
+            (wf : bsigs; bsig ⊢ b WF-cont) :
+            (bsigs ++ bsigs'); bsig ⊢ b WF-cont :=
       wf.cast0.weakening_bsigs.cast0
   end WF
 
   theorem WFRets0_iff_WF {bsigs : BlockSigs} {bsig : BlockSig} {b : Cont} :
-                         WFRets bsigs bsig 0 b ↔ WF bsigs bsig b :=
+                         bsigs; bsig ⊢ b(0) WF-cont ↔ bsigs; bsig ⊢ b WF-cont :=
     ⟨Coe.coe, Coe.coe⟩
-
-  deriving instance DecidableEq for Cont
 end Cont
 
 namespace Code
   --notation e:arg " ;; " c => stmt e c
 
-  inductive WF (fsigs : FuncSigs) (bsigs ret) : BlockSig -> Code -> Prop where
+  inductive WF (fsigs : FuncSigs) (bsigs: BlockSigs) : BlockSig -> Code -> Prop where
     | stmt
         {bsig : BlockSig}
         {e : Expr}
         {c : Code} :
-        e.WF bsig.arity ->
-        c.WF fsigs bsigs ret bsig.bind ->
-        (stmt e c).WF fsigs bsigs ret bsig
+        bsig.arity ⊢ e WF-expr ->
+        c.WF fsigs bsigs bsig.bind ->
+        (stmt e c).WF fsigs bsigs bsig
 
     | goto
         {bsig : BlockSig}
         {bnext : Cont} :
-        bnext.WF bsigs bsig ->
-        (goto bnext).WF fsigs bsigs ret bsig
+        bsigs; bsig ⊢ bnext WF-cont ->
+        (goto bnext).WF fsigs bsigs bsig
 
     | ite
         {bsig : BlockSig}
         {cond : Atom}
         {bthen : Cont}
         {belse : Cont} :
-        cond.WF bsig.arity ->
-        bthen.WF bsigs bsig ->
-        belse.WF bsigs bsig ->
-        (ite cond bthen belse).WF fsigs bsigs ret bsig
+        bsig.arity ⊢ cond WF-atom ->
+        bsigs; bsig ⊢ bthen WF-cont ->
+        bsigs; bsig ⊢ belse WF-cont ->
+        (ite cond bthen belse).WF fsigs bsigs bsig
 
     | call
         {bsig : BlockSig}
@@ -285,185 +460,175 @@ namespace Code
         {bret : Cont} :
         (_ : f < fsigs.length) ->
         fsigs[f].arity = args.length ->
-        IVec (·.WF bsig.arity) args ->
-        bret.WFRets bsigs bsig fsigs[f].ret ->
-        (call f args bret).WF fsigs bsigs ret bsig
+        IVec (bsig.arity ⊢ · WF-var) args ->
+        bsigs; bsig ⊢ bret(fsigs[f].ret) WF-cont ->
+        (call f args bret).WF fsigs bsigs bsig
         
     | retn
         {bsig : BlockSig}
         {args : List Var} :
-        bsig.sporkNest = [] ->
-        ret = args.length ->
-        IVec (·.WF bsig.arity) args ->
-        (retn args).WF fsigs bsigs ret bsig
+        bsig.oblg = .retn args.length ->
+        IVec (bsig.arity ⊢ · WF-var) args ->
+        (retn args).WF fsigs bsigs bsig
 
     | spork
         {bsig : BlockSig}
         {bbody : Cont}
-        {fspwn : FuncIdx}
-        {args : List Var} :
-        (_ : fspwn < fsigs.length) ->
-        fsigs[fspwn].arity = args.length ->
-        IVec (·.WF bsig.arity) args ->
-        bbody.WF bsigs (bsig.spork fsigs[fspwn].ret) ->
-        (spork bbody fspwn args).WF fsigs bsigs ret bsig
+        {bspwn : Cont}
+        {n : Nat} :
+        bsigs; (bsig.spoin n) ⊢ bbody WF-cont ->
+        bsigs; (bsig.exit n) ⊢ bspwn WF-cont ->
+        (spork n bbody bspwn).WF fsigs bsigs bsig
 
     | spoin
         {bsig : BlockSig}
         {bunpr : Cont}
         {bprom : Cont} :
-        (bsig_sn_nonnil : bsig.sporkNest ≠ []) ->
-        bunpr.WF bsigs bsig.spoin ->
-        bprom.WFRets bsigs bsig.spoin (bsig.sporkNest.head bsig_sn_nonnil) ->
-        (spoin bunpr bprom).WF fsigs bsigs ret bsig
-
-
-  @[simp] def split : Code -> List Expr × (c : Code) ×' (∀ e, ∀ c', c ≠ .stmt e c')
-    | stmt e c => let (es, cp) := c.split; (e :: es, cp)
-    | goto bnext => ([], ⟨goto bnext, by intros e c; simp⟩)
-    | ite e bthen belse => ([], ⟨ite e bthen belse, by intros e c; simp⟩)
-    | call g args bret => ([], ⟨call g args bret, by intros e c; simp⟩)
-    | retn args => ([], ⟨retn args, by intros e c; simp⟩)
-    | spork bbody gspwn gargs => ([], ⟨spork bbody gspwn gargs, by intros e c; simp⟩)
-    | spoin bunpr bprom => ([], ⟨spoin bunpr bprom, by intros e c; simp⟩)
-
-  @[simp] def join : List Expr -> Code -> Code
-    | [], c => c
-    | e :: es, c => stmt e (join es c)
-
-  @[simp] theorem join_split {c e c' p} (q : split c = (e, ⟨c', p⟩)) : join e c' = c := by
-    cases c <;> try (cases e <;> simp_all)
-    · case stmt e' es' e'' es'' =>
-      exact join_split (Prod.ext q.1.2 q.2)
+        bsig.oblg.isSpoin ->
+        bsigs; bsig.tail ⊢ bunpr WF-cont ->
+        bsigs; (bsig.tail.join bsig.head) ⊢ bprom WF-cont ->
+        (spoin bunpr bprom).WF fsigs bsigs bsig
+    
+    | join
+        {bsig : BlockSig}
+        {bsync : Cont} :
+        bsig.oblg.isJoin ->
+        bsync.WFRets bsigs bsig.tail bsig.head ->
+        (join bsync).WF fsigs bsigs bsig
+    
+    | exit
+        {bsig : BlockSig}
+        {args : List Var}:
+        bsig.oblg = .exit args.length ->
+        IVec (bsig.arity ⊢ · WF-var) args ->
+        (exit args).WF fsigs bsigs bsig
 
   namespace WF
-    instance instDecidable {fsigs bsigs ret bsig} : (c : Code) ->
-                           Decidable (c.WF fsigs bsigs ret bsig)
+    
+    notation (name := notationwf) fsigs:arg " ; " bsigs:arg " ; " bsig:arg " ⊢ " c:arg " WF-code" => WF fsigs bsigs bsig c
+--    notation:min (name := notationwf') fsigs:arg bsigs:arg bsig:arg " ⊢ " c " WF-code" => WF fsigs bsigs bsig c
+
+    instance instDecidable {fsigs bsigs bsig} : (c : Code) ->
+                           Decidable (fsigs; bsigs; bsig ⊢ c WF-code)
       | .stmt e c =>
-          let _ : Decidable (c.WF fsigs bsigs ret bsig.bind) := instDecidable c
-          decidable_of_iff (e.WF bsig.arity ∧ c.WF fsigs bsigs ret bsig.bind)
+          let _ : Decidable (fsigs; bsigs; bsig.bind ⊢ c WF-code) := instDecidable c;
+          decidable_of_iff (bsig.arity ⊢ e WF-expr ∧
+                            fsigs; bsigs; bsig.bind ⊢ c WF-code)
             ⟨λ ⟨e, c⟩ => stmt e c, λ | stmt e c => ⟨e, c⟩⟩
       | .goto bnext =>
-          decidable_of_iff (bnext.WF bsigs bsig)
+          decidable_of_iff (bsigs; bsig ⊢ bnext WF-cont)
             ⟨goto, λ | goto wf => wf⟩
       | .ite cond bthen belse =>
-          decidable_of_iff (cond.WF bsig.arity ∧ bthen.WF bsigs bsig ∧ belse.WF bsigs bsig)
+          decidable_of_iff (bsig.arity ⊢ cond WF-atom ∧
+                            bsigs; bsig ⊢ bthen WF-cont ∧
+                            bsigs; bsig ⊢ belse WF-cont)
             ⟨λ ⟨a, b, c⟩ => ite a b c, λ | ite a b c => ⟨a, b, c⟩⟩
       | .call f args bret =>
           decidable_of_iff (∃ _ : f < fsigs.length,
                             fsigs[f].arity = args.length ∧
-                            IVec (·.WF bsig.arity) args ∧
-                            bret.WFRets bsigs bsig fsigs[f].ret)
+                            IVec (bsig.arity ⊢ · WF-var) args ∧
+                            bsigs; bsig ⊢ bret(fsigs[f].ret) WF-cont)
             ⟨λ ⟨a, b, c, d⟩ => call a b c d,
              λ | call a b c d => ⟨a, b, c, d⟩⟩
       | .retn args =>
-          decidable_of_iff (bsig.sporkNest = [] ∧ ret = args.length ∧ IVec (·.WF bsig.arity) args)
-            ⟨λ ⟨a, b, c⟩ => retn a b c, λ | retn a b c => ⟨a, b, c⟩⟩
-      | .spork bbody fspwn args =>
-          decidable_of_iff (∃ _ : fspwn < fsigs.length,
-                            fsigs[fspwn].arity = args.length ∧
-                            IVec (·.WF bsig.arity) args ∧
-                            bbody.WF bsigs (bsig.spork fsigs[fspwn].ret))
-            ⟨λ ⟨a, b, c, d⟩ => spork a b c d, λ | spork a b c d => ⟨a, b, c, d⟩⟩
+          decidable_of_iff (bsig.oblg = Oblg.retn args.length ∧
+                            IVec (bsig.arity ⊢ · WF-var) args)
+            ⟨λ ⟨a, b⟩ => retn a b, λ | retn a b => ⟨a, b⟩⟩
+      | .spork n bbody bspwn =>
+          decidable_of_iff (bsigs; (bsig.spoin n) ⊢ bbody WF-cont ∧
+                            bsigs; (bsig.exit n) ⊢ bspwn WF-cont)
+            ⟨λ ⟨a, b⟩ => spork a b, λ | spork a b => ⟨a, b⟩⟩
       | .spoin bunpr bprom =>
-          match (generalizing := true) h : bsig with
-            | ⟨arity, []⟩ =>
-                isFalse (λ x => by cases x <;> contradiction)
-            | ⟨arity, s :: ss⟩ =>
-                decidable_of_iff (bunpr.WF bsigs ⟨arity, ss⟩ ∧
-                                  bprom.WFRets bsigs ⟨arity, ss⟩ s)
-                ⟨λ ⟨a, b⟩ => spoin (by simp) a b,
-                 λ | spoin h' a b => ⟨a, b⟩⟩
+          decidable_of_iff (bsig.oblg.isSpoin ∧
+                            bsigs; bsig.tail ⊢ bunpr WF-cont ∧
+                            bsigs; (bsig.tail.join bsig.head) ⊢ bprom WF-cont)
+            ⟨λ ⟨a, b, c⟩ => spoin a b c, λ | spoin a b c => ⟨a, b, c⟩⟩
+      | .join bsync =>
+          decidable_of_iff (bsig.oblg.isJoin ∧
+                            bsync.WFRets bsigs bsig.tail bsig.head)
+            ⟨λ ⟨a, b⟩ => join a b, λ | join a b => ⟨a, b⟩⟩
+      | .exit args =>
+          decidable_of_iff (bsig.oblg = .exit args.length ∧
+                            IVec (bsig.arity ⊢ · WF-var) args)
+            ⟨λ ⟨a, b⟩ => exit a b, λ | exit a b => ⟨a, b⟩⟩
 
     -- Accessor methods
-    theorem stmt_expr {fsigs bsigs ret bsig e c} : (Code.stmt e c).WF fsigs bsigs ret bsig -> e.WF bsig.arity
+    theorem stmt_expr {fsigs bsigs bsig e c} : fsigs; bsigs; bsig ⊢ (.stmt e c) WF-code -> bsig.arity ⊢ e WF-expr
       | stmt ewf _cwf => ewf
-    theorem stmt_code {fsigs bsigs ret bsig e c} : (Code.stmt e c).WF fsigs bsigs ret bsig -> c.WF fsigs bsigs ret bsig.bind
+    theorem stmt_code {fsigs bsigs bsig e c} : fsigs; bsigs; bsig ⊢ (.stmt e c) WF-code -> fsigs; bsigs; bsig.bind ⊢ c WF-code
       | stmt _ewf cwf => cwf
 
-    theorem goto_bnext {fsigs bsigs ret bsig bnext} :
-                       WF fsigs bsigs ret bsig (.goto bnext) ->
-                       bnext.WF bsigs bsig
+    theorem goto_bnext {fsigs bsigs bsig bnext} :
+                       fsigs; bsigs; bsig ⊢ (.goto bnext) WF-code ->
+                       bsigs; bsig ⊢ bnext WF-cont
       | goto bnextwf => bnextwf
 
-    theorem ite_cond {fsigs bsigs ret bsig cond bthen belse} :
-                     WF fsigs bsigs ret bsig (.ite cond bthen belse) ->
-                     cond.WF bsig.arity
+    theorem ite_cond {fsigs bsigs bsig cond bthen belse} :
+                     fsigs; bsigs; bsig ⊢ (.ite cond bthen belse) WF-code ->
+                     bsig.arity ⊢ cond WF-atom
       | ite condwf _ _ => condwf
-    theorem ite_bthen {fsigs bsigs ret bsig cond bthen belse} :
-                      WF fsigs bsigs ret bsig (.ite cond bthen belse) ->
-                      bthen.WF bsigs bsig
+    theorem ite_bthen {fsigs bsigs bsig cond bthen belse} :
+                      fsigs; bsigs; bsig ⊢ (.ite cond bthen belse) WF-code ->
+                      bsigs; bsig ⊢ bthen WF-cont
       | ite _ bthenwf _ => bthenwf
-    theorem ite_belse {fsigs bsigs ret bsig cond bthen belse} :
-                      WF fsigs bsigs ret bsig (.ite cond bthen belse) ->
-                      belse.WF bsigs bsig
+    theorem ite_belse {fsigs bsigs bsig cond bthen belse} :
+                      fsigs; bsigs; bsig ⊢ (.ite cond bthen belse) WF-code ->
+                      bsigs; bsig ⊢ belse WF-cont
       | ite _ _ belsewf => belsewf
 
-    theorem call_flt {fsigs bsigs ret bsig f args bret} :
-                     WF fsigs bsigs ret bsig (.call f args bret) ->
+    theorem call_flt {fsigs bsigs bsig f args bret} :
+                     fsigs; bsigs; bsig ⊢ (.call f args bret) WF-code ->
                      f < fsigs.length
       | call flt _ _ _ => flt
-    theorem call_arity {fsigs bsigs ret bsig f args bret} :
-                       (wf : WF fsigs bsigs ret bsig (.call f args bret)) ->
+    theorem call_arity {fsigs bsigs bsig f args bret} :
+                       (wf : fsigs; bsigs; bsig ⊢ (.call f args bret) WF-code) ->
                        (fsigs[f]'wf.call_flt).arity = args.length
       | call _ aritywf _ _ => aritywf
-    theorem call_args {fsigs bsigs ret bsig f args bret} :
-                      WF fsigs bsigs ret bsig (.call f args bret) ->
-                      IVec (·.WF bsig.arity) args
+    theorem call_args {fsigs bsigs bsig f args bret} :
+                      fsigs; bsigs; bsig ⊢ (.call f args bret) WF-code ->
+                      IVec (bsig.arity ⊢ · WF-var) args
       | call _ _ argswf _ => argswf
-    theorem call_bret {fsigs bsigs ret bsig f args bret} :
-                      (wf : WF fsigs bsigs ret bsig (.call f args bret)) ->
-                      bret.WFRets bsigs bsig (fsigs[f]'wf.call_flt).ret
+    theorem call_bret {fsigs bsigs bsig f args bret} :
+                      (wf : fsigs; bsigs; bsig ⊢ (.call f args bret) WF-code) ->
+                      bsigs; bsig ⊢ bret((fsigs[f]'wf.call_flt).ret) WF-cont
       | call _ _ _ bretwf => bretwf
 
-    theorem retn_sn_nil {fsigs bsigs ret bsig args} :
-                          WF fsigs bsigs ret bsig (.retn args) ->
-                          bsig.sporkNest = []
-      | retn n _ _ => n
-    theorem retn_length {fsigs bsigs ret bsig args} :
-                        WF fsigs bsigs ret bsig (.retn args) ->
-                        ret = args.length
-      | retn _ l _ => l
-    theorem retn_args {fsigs bsigs ret bsig args} :
-                      WF fsigs bsigs ret bsig (.retn args) ->
-                      IVec (·.WF bsig.arity) args
-      | retn _ _ a => a
+    theorem retn_oblg {fsigs bsigs bsig args} :
+                      fsigs; bsigs; bsig ⊢ (.retn args) WF-code ->
+                      bsig.oblg = .retn args.length
+      | retn n _ => n
+    theorem retn_args {fsigs bsigs bsig args} :
+                      fsigs; bsigs; bsig ⊢ (.retn args) WF-code ->
+                      IVec (bsig.arity ⊢ · WF-var) args
+      | retn _ a => a
 
-    theorem spork_flt {fsigs bsigs ret bsig bbody f args} :
-                      WF fsigs bsigs ret bsig (.spork bbody f args) ->
-                      f < fsigs.length
-      | spork flt _ _ _ => flt
-    theorem spork_arity {fsigs bsigs ret bsig bbody f args} :
-                        (wf : WF fsigs bsigs ret bsig (.spork bbody f args)) ->
-                        (fsigs[f]'wf.spork_flt).arity = args.length
-      | spork _ aritywf _ _ => aritywf
-    theorem spork_args {fsigs bsigs ret bsig bbody f args} :
-                      WF fsigs bsigs ret bsig (.spork bbody f args) ->
-                      IVec (·.WF bsig.arity) args
-      | spork _ _ argswf _ => argswf
-    theorem spork_bbody {fsigs bsigs ret bsig bbody f args} :
-                        (wf : WF fsigs bsigs ret bsig (.spork bbody f args)) ->
-                        bbody.WF bsigs (bsig.spork (fsigs[f]'wf.spork_flt).ret)
-      | spork _ _ _ bbodywf => bbodywf
+    theorem spork_bbody {fsigs bsigs bsig n bbody bspwn} :
+                        (wf : fsigs; bsigs; bsig ⊢ (.spork n bbody bspwn) WF-code) ->
+                        bsigs; (bsig.spoin n) ⊢ bbody WF-cont
+      | spork bbodywf _ => bbodywf
 
-    theorem spoin_sn_nonnil {fsigs bsigs ret bsig bunpr bprom} :
-                            WF fsigs bsigs ret bsig (.spoin bunpr bprom) ->
-                            bsig.sporkNest ≠ []
-      | spoin nn _ _ => nn
-    theorem spoin_bunpr {fsigs bsigs ret bsig bunpr bprom} :
-                        WF fsigs bsigs ret bsig (.spoin bunpr bprom) ->
-                        bunpr.WF bsigs bsig.spoin
+    theorem spork_bspwn {fsigs bsigs bsig n bbody bspwn} :
+                        (wf : fsigs; bsigs; bsig ⊢ (.spork n bbody bspwn) WF-code) ->
+                        bsigs; (bsig.exit n) ⊢ bspwn WF-cont
+      | spork _ bspwnwf => bspwnwf
+
+    theorem spoin_oblg {fsigs bsigs bsig bunpr bprom} :
+                       fsigs; bsigs; bsig ⊢ (.spoin bunpr bprom) WF-code ->
+                       bsig.oblg.isSpoin
+      | spoin issp _ _ => issp
+    theorem spoin_bunpr {fsigs bsigs bsig bunpr bprom} :
+                        fsigs; bsigs; bsig ⊢ (.spoin bunpr bprom) WF-code ->
+                        bsigs; bsig.tail ⊢ bunpr WF-cont
       | spoin _ bunprwf _ => bunprwf
-    theorem spoin_bprom {fsigs bsigs ret bsig bunpr bprom} :
-                        (wf : WF fsigs bsigs ret bsig (.spoin bunpr bprom)) ->
-                        bprom.WFRets bsigs bsig.spoin
-                          (bsig.sporkNest.head wf.spoin_sn_nonnil)
+    theorem spoin_bprom {fsigs bsigs bsig bunpr bprom} :
+                        (wf : fsigs; bsigs; bsig ⊢ (.spoin bunpr bprom) WF-code) ->
+                        bsigs; (bsig.tail.join bsig.head) ⊢ bprom WF-cont
       | spoin _ _ bpromwf => bpromwf
 
     theorem weakening_bsigs
-            {fsigs bsigs bsigs' ret bsig c} :
-            WF fsigs bsigs ret bsig c ->
-            WF fsigs (bsigs ++ bsigs') ret bsig c
+            {fsigs bsigs bsigs' bsig c} :
+            fsigs; bsigs; bsig ⊢ c WF-code ->
+            fsigs; (bsigs ++ bsigs'); bsig ⊢ c WF-code
       | stmt ewf cwf =>
         stmt ewf cwf.weakening_bsigs
       | goto bnextwf =>
@@ -472,22 +637,26 @@ namespace Code
         ite ewf bthenwf.weakening_bsigs belsewf.weakening_bsigs
       | call flt aritywf argswf bretwf =>
         call flt aritywf argswf bretwf.weakening_bsigs
-      | retn snwf retwf argswf =>
-        retn snwf retwf argswf
-      | spork flt aritywf argswf bbodywf =>
-        spork flt aritywf argswf bbodywf.weakening_bsigs
+      | retn oblg argswf =>
+        retn oblg argswf
+      | spork bbodywf bspwnwf =>
+        spork bbodywf.weakening_bsigs bspwnwf.weakening_bsigs
       | spoin snwf bunprwf bpromwf =>
         spoin snwf bunprwf.weakening_bsigs bpromwf.weakening_bsigs
+      | join oblg bsyncwf =>
+        join oblg bsyncwf.weakening_bsigs
+      | exit oblg argswf =>
+        exit oblg argswf
 
-    theorem join_wf {fsigs bsigs ret bsig} :
+    theorem merge_wf {fsigs bsigs bsig} :
             {e : List Expr} -> {c : Code} ->
-            (∀ i : Fin e.length, e[i].WF (bsig.arity + i)) ->
-            c.WF fsigs bsigs ret (bsig + .mk e.length []) ->
-            (c.join e).WF fsigs bsigs ret bsig
+            (∀ i : Fin e.length, (bsig.arity + i) ⊢ e[i] WF-expr) ->
+            fsigs; bsigs; (bsig.binds e.length) ⊢ c WF-code ->
+            fsigs; bsigs; bsig ⊢ (c.merge e) WF-code
       | [], c, ewf, cwf => by simpa using cwf
       | e :: es, c, ewf, cwf =>
         .stmt (ewf ⟨0, by simp⟩)
-          (join_wf (bsig := bsig.bind) (e := es)
+          (merge_wf (bsig := bsig.bind) (e := es)
             (λ i => let ewf' := ewf ⟨i.1 + 1, by simp⟩
                     by simp[← Nat.add_assoc bsig.1 1 i.1] at ewf'
                        simp
@@ -501,12 +670,12 @@ namespace Code
                    ← Nat.add_assoc] at cwf
                 exact cwf))
 
-    theorem split_wf {fsigs bsigs ret bsig} {c : Code} (cwf : c.WF fsigs bsigs ret bsig) :
-            (∀ i : Fin c.split.1.length, c.split.1[i].WF (bsig.arity + i))
-              ∧ c.split.2.1.WF fsigs bsigs ret (bsig + .mk c.split.1.length []) := by
+    theorem split_wf {fsigs bsigs bsig} {c : Code} (cwf : fsigs; bsigs; bsig ⊢ c WF-code) :
+            (∀ i : Fin c.split.1.length, (bsig.arity + i) ⊢ c.split.1[i] WF-expr)
+              ∧ fsigs; bsigs; (bsig.binds c.split.1.length) ⊢ c.split.2.1 WF-code := by
       cases c <;> try (exact And.intro (λ i => nomatch i) (by simpa using cwf))
       · case stmt e c =>
-        let p := @split_wf fsigs bsigs ret bsig.bind c cwf.stmt_code
+        let p := @split_wf fsigs bsigs bsig.bind c cwf.stmt_code
         apply And.intro
         · exact (λ | ⟨0, l⟩ => cwf.stmt_expr
                    | ⟨i + 1, l⟩ =>
@@ -517,119 +686,112 @@ namespace Code
                simpa[h, Nat.add_assoc, Nat.add_comm 1]
                using p.2)
   end WF
-
-  deriving instance DecidableEq for Code
 end Code
 
 namespace Block
-  @[simp] abbrev bsig | mk bsig _code => bsig
-  @[simp] abbrev code | mk _bsig code => code
-
-  inductive WF (fsigs bsigs ret) (b : Block) : Prop where
-    | mk (c : b.code.WF fsigs bsigs ret b.bsig)
+  inductive WF (fsigs bsigs) (b : Block) : Prop where
+    | mk (c : b.code.WF fsigs bsigs b.bsig)
 
   namespace WF
-    instance (fsigs bsigs ret) : {b : Block} -> Decidable (b.WF fsigs bsigs ret)
+    notation (name := notationwf) fsigs:arg " ; " bsigs:arg " ⊢ " b:arg " WF-block" => WF fsigs bsigs b
+
+    instance (fsigs bsigs) : {b : Block} -> Decidable (fsigs; bsigs ⊢ b WF-block)
       | .mk bsig code =>
-        decidable_of_iff (code.WF fsigs bsigs ret bsig)
+        decidable_of_iff (fsigs; bsigs; bsig ⊢ code WF-code)
           ⟨λ a => mk a, λ | mk a => a⟩
 
-    theorem code {fsigs bsigs ret b} : WF fsigs bsigs ret b ->
-                 b.code.WF fsigs bsigs ret b.bsig
+    theorem code {fsigs bsigs b} : fsigs; bsigs ⊢ b WF-block ->
+                 fsigs; bsigs; b.bsig ⊢ b.code WF-code
       | .mk c => c
 
     theorem weakening_bsigs
-            {fsigs bsigs bsigs' ret b} :
-            WF fsigs bsigs ret b ->
-            WF fsigs (bsigs ++ bsigs') ret b
+            {fsigs bsigs bsigs' b} :
+            fsigs; bsigs ⊢ b WF-block ->
+            fsigs; (bsigs ++ bsigs') ⊢ b WF-block
       | mk cwf => mk cwf.weakening_bsigs
   end WF
-
-  deriving instance DecidableEq for Block
-
-  instance : Inhabited Block where
-    default := mk ⟨0, []⟩ (.retn [])
 end Block
 
-namespace Func
-  @[simp] abbrev fsig | mk fsig _blocks => fsig
-  @[simp] abbrev blocks | mk _fsig blocks => blocks
-  @[simp] abbrev bsigs : Func -> BlockSigs | mk _fsig blocks => blocks.map (·.bsig)
-  @[simp] abbrev size | mk _fsig blocks => blocks.length
-  
-  @[simp] theorem size_eq_bsigs_length (f : Func) : f.bsigs.length = f.size :=
-    by simp
-
-  inductive WF (fsigs : FuncSigs) (f : Func) : Prop where
-    | mk (blocks : IVec (·.WF fsigs (f.blocks.map (·.bsig)) f.fsig.ret) f.blocks)
-         (head : HeadIs f.blocks (·.bsig) ⟨f.fsig.arity, []⟩)
+namespace Blocks
+  inductive WF (fsigs : FuncSigs) (bs: List Block) (bsig: BlockSig) : Prop where
+    | mk (blocks : IVec (fsigs; (bs.map (·.bsig)) ⊢ · WF-block) bs)
+         (head : HeadIs bs (·.bsig) bsig)
 
   namespace WF
-    instance {fsigs : FuncSigs} : {f : Func} -> Decidable (f.WF fsigs)
-      | .mk fsig blocks => decidable_of_iff
-          (IVec (·.WF fsigs (blocks.map (·.bsig)) fsig.ret) blocks ∧
-           HeadIs blocks (·.bsig) ⟨fsig.arity, []⟩)
-          ⟨λ ⟨a, b⟩ => mk a b, λ | mk a b => ⟨a, b⟩⟩
+    notation (name := notationwf) fsigs:arg " ; " bsig:arg " ⊢ " bs:arg " WF-blocks" => WF fsigs bs bsig
 
-    theorem blocks {fsigs f} : WF fsigs f -> IVec (·.WF fsigs (f.blocks.map (·.bsig)) f.fsig.ret) f.blocks
-      | mk blocks _head => blocks
-    theorem head {fsigs f} : WF fsigs f -> HeadIs f.blocks (·.bsig) ⟨f.fsig.arity, []⟩
-      | mk _blocks head => head
+    instance wf {fsigs: FuncSigs} {bs: List Block} {bsig: BlockSig}:
+                      Decidable (fsigs; bsig ⊢ bs WF-blocks) :=
+      decidable_of_iff (IVec (fsigs; (bs.map (·.bsig)) ⊢ · WF-block) bs ∧
+                        HeadIs bs (·.bsig) bsig)
+        ⟨λ ⟨a, b⟩ => mk a b, λ | mk a b => ⟨a, b⟩⟩
+
+    theorem blocks {fsigs bs bsig} : fsigs; bsig ⊢ bs WF-blocks -> IVec (fsigs; (bs.map (·.bsig)) ⊢ · WF-block) bs
+      | .mk blocks _head => blocks
+    theorem head {fsigs bs bsig} : fsigs; bsig ⊢ bs WF-blocks -> HeadIs bs (·.bsig) bsig
+      | .mk _blocks head => head
+
+    theorem add_blocks
+            {fsigs bs bs' bsig} :
+            fsigs; bsig ⊢ bs WF-blocks ->
+            IVec (fsigs; ((bs ++ bs').map (·.bsig)) ⊢ · WF-block) bs' ->
+            fsigs; bsig ⊢ (bs ++ bs') WF-blocks
+      | .mk blocks head, bs'wf =>
+        .mk (IVec.append (blocks.map
+              (λ b bwf => by simpa using bwf.weakening_bsigs)) bs'wf)
+            ⟨by rw[List.head?_eq_some_head,
+                   List.head_append_left head.nonnil,
+                   ← head.head?eq,
+                   List.head?_eq_head head.nonnil]⟩
+  end WF
+end Blocks
+
+namespace Func
+  -- inductive WF (fsigs : FuncSigs) (f : Func) : Prop where
+  --   | mk (blocks : IVec (·.WF fsigs (f.blocks.map (·.bsig))) f.blocks)
+  --        (head : HeadIs f.blocks (·.bsig) ⟨f.fsig.arity, .retn f.fsig.ret⟩)
+  abbrev WF (fsigs: FuncSigs) (f: Func): Prop :=
+    fsigs; ⟨f.fsig.arity, .retn f.fsig.ret⟩ ⊢ f.blocks WF-blocks
+
+  namespace WF
+    notation (name := notationwf) fsigs:arg " ⊢ " f:arg " WF-func" => WF fsigs f
+    notation (name := notationwf') P:arg " ⊢ " f:arg " WF-func'" => WF (Program.fsigs P) f
+    
+    instance {fsigs : FuncSigs} {f : Func}: Decidable (fsigs ⊢ f WF-func) := Blocks.WF.wf
+
+    theorem blocks {fsigs f} : fsigs ⊢ f WF-func ->
+                   IVec (fsigs; (f.blocks.map (·.bsig)) ⊢ · WF-block) f.blocks
+      := Blocks.WF.blocks
+    theorem head {fsigs f} : fsigs ⊢ f WF-func ->
+                 HeadIs f.blocks (·.bsig) ⟨f.fsig.arity, .retn f.fsig.ret⟩
+      := Blocks.WF.head
 
     theorem add_blocks
             {fsigs fsig bs bs'} :
-            WF fsigs (.mk fsig bs) ->
-            IVec (·.WF fsigs ((bs ++ bs').map (·.bsig)) fsig.ret) bs' ->
-            WF fsigs (.mk fsig (bs ++ bs'))
-      | mk blocks head, bs'wf =>
-        mk (IVec.append (blocks.map
-             (λ b bwf => by simpa using bwf.weakening_bsigs)) bs'wf)
-           ⟨by rw[List.head?_eq_some_head,
-                  List.head_append_left head.nonnil,
-                  ← head.head?eq,
-                  List.head?_eq_head head.nonnil]⟩
+            fsigs ⊢ (.mk fsig bs) WF-func ->
+            IVec (fsigs; ((bs ++ bs').map (·.bsig)) ⊢ · WF-block) bs' ->
+            fsigs ⊢ (.mk fsig (bs ++ bs')) WF-func :=
+      Blocks.WF.add_blocks
   end WF
-
-  deriving instance DecidableEq for Func
-
-  instance : Inhabited Func where
-    default := mk ⟨0, 0⟩ default
-
-  instance : GetElem Func BlockIdx Block (λ f b => b < f.blocks.length) where
-    getElem f b p := f.blocks[b]
 end Func
 
 namespace Program
-  @[simp] abbrev funs | mk funs => funs
-  @[simp] abbrev fsigs : Program -> FuncSigs | mk funs => funs.map (·.fsig)
-  @[simp] abbrev size | mk funs => funs.length
-
-  @[simp] theorem size_eq_fsigs_length (P : Program) : P.fsigs.length = P.size :=
-    by simp
-
   inductive WF (P : Program): Prop where
-    | mk (funcs : IVec (·.WF P.fsigs) P.funs)
-         (head : HeadIs P.funs (·.fsig) ⟨0, 1⟩)
+    | mk (funcs : IVec (P ⊢ · WF-func') P.funs)
+         (main: P.fsigs; ⟨0, .exit 1⟩ ⊢ P.main WF-blocks)
 
   namespace WF
-    instance : {p : Program} -> Decidable p.WF
-      | .mk funs => decidable_of_iff
-          (IVec (·.WF (funs.map (·.fsig))) funs ∧
-           HeadIs funs (·.fsig) ⟨0, 1⟩)
+    notation (name := notationwf) P:arg " WF-program" => WF P
+    
+    instance {P : Program}: Decidable (P WF-program) :=
+      decidable_of_iff (IVec (P.fsigs ⊢ · WF-func) P.funs ∧
+                        P.fsigs; ⟨0, .exit 1⟩ ⊢ P.main WF-blocks)
           ⟨λ ⟨a, b⟩ => mk a b, λ | mk a b => ⟨a, b⟩⟩
 
-    theorem funcs {P} : WF P -> IVec (·.WF P.fsigs) P.funs | .mk funcs _head => funcs
-    theorem head {P} : WF P -> HeadIs P.funs (·.fsig) ⟨0, 1⟩ | .mk _funcs head => head
-    theorem main_lt : {P : Program} -> WF P -> 0 < P.fsigs.length
-      | .mk (main :: funs), .mk funcs head => by simp
-    theorem main_lt' : {P : Program} -> WF P -> 0 < P.size
-      | .mk (main :: funs), .mk funcs head => by simp
-  end WF
-
-  deriving instance DecidableEq for Program
-
-  instance : GetElem Program FuncIdx Func (λ P f => f < P.size) where
-    getElem P f p := P.funs[f]
-  
+    theorem funcs {P} : P WF-program -> IVec (P.fsigs ⊢ · WF-func) P.funs
+      | .mk funcs _main => funcs
+    theorem main {P} : P WF-program -> P.fsigs; ⟨0, .exit 1⟩ ⊢ P.main WF-blocks
+      | mk _funcs main => main
+  end WF  
 end Program
 
